doc/coq/Linking.v
@@ -1,6 +1,112 @@
-From MODULAR Require Import Concrete.
+From MODULAR Require Export Sound.
 
-Fixpoint inject_ctx Cout Cin :=
+(* before, after *)
+Generalizable Variables BT AT.
+
+Inductive link `{OrderT BT} `{OrderT AT} :=
+  | BF (t : BT)
+  | AF (t : AT)
+.
+
+Definition link_leb `{OrderT BT} `{OrderT AT} (t1 : link) (t2 : link) :=
+  match t1, t2 with
+  | BF t1, BF t2 => leb t1 t2
+  | AF t1, AF t2 => leb t1 t2
+  | BF t1, AF t2 => true
+  | AF t1, BF t2 => false
+  end.
+
+Definition link_eqb `{OrderT BT} `{OrderT AT} (t1 : link) (t2 : link) :=
+  match t1, t2 with
+  | BF t1, BF t2 => eqb t1 t2
+  | AF t1, AF t2 => eqb t1 t2
+  | _, _ => false  
+  end.
+
+Lemma link_leb_refl : 
+  forall `{OrderT BT} `{OrderT AT} t,
+  link_leb t t = true.
+Proof.
+  intros. destruct t; apply leb_refl.
+Qed.
+
+Lemma link_leb_trans :
+  forall `{OrderT BT} `{OrderT AT} t t' t''
+         (LE : link_leb t t' = true)
+         (LE' : link_leb t' t'' = true),
+  link_leb t t'' = true.
+Proof.
+  intros.
+  destruct t; destruct t'; destruct t'';
+  simpl in *;
+  try apply leb_trans with (t' := t0);
+  try inversion LE;
+  try inversion LE';
+  eauto.
+Qed.
+
+Lemma link_leb_sym :
+  forall `{OrderT BT} `{OrderT AT} t t'
+         (LE : link_leb t t' = true)
+         (LE' : link_leb t' t = true),
+  t = t'.
+Proof.
+  intros.
+  destruct t; destruct t';
+  simpl in *;
+  try inversion LE;
+  try inversion LE';
+  assert (t = t0) as RR;
+  try apply leb_sym; eauto;
+  rewrite RR; eauto.
+Qed.
+
+Lemma link_eqb_eq :
+  forall `{OrderT BT} `{OrderT AT} t t',
+  link_eqb t t' = true <-> t = t'.
+Proof.
+  intros.
+  destruct t; destruct t';
+  simpl in *;
+  split; intro EQ;
+  try rewrite eqb_eq in *;
+  try inversion EQ;
+  subst; eauto.
+Qed.
+
+Lemma link_eqb_neq :
+  forall `{OrderT BT} `{OrderT AT} t t',
+  link_eqb t t' = false <-> t <> t'.
+Proof.
+  intros.
+  destruct t; destruct t';
+  simpl in *;
+  split; intro NEQ;
+  try rewrite eqb_neq in *;
+  try inversion NEQ;
+  subst; unfold not in *;
+  try intros contra;
+  try apply NEQ;
+  try inversion contra;
+  eauto.
+Qed.
+
+#[export] Instance LinkOrderT `{OrderT BT} `{OrderT AT} : OrderT link:=
+  {
+    leb := link_leb;
+    leb_refl := link_leb_refl;
+    leb_trans := link_leb_trans;
+    leb_sym := link_leb_sym;
+    eqb := link_eqb;
+    eqb_eq := link_eqb_eq;
+    eqb_neq := link_eqb_neq
+  }.
+
+Definition filter_mem 
+  `{BO : OrderT BT} `{AO : OrderT AT} `{OrderT (@link )}
+  (mem : BT -> option (@expr_value BT)) := 1.
+
+Fixpoint inject_ctx `{OrderT T1}Cout Cin :=
   match Cin with
   | ([||]) => Cout
   | dy_c_lam x t C' =>
